theories/simplang/class_instances.v
@@ -32,7 +32,7 @@ Section irreducible.
     let IH := fresh "IH" in
     let Ki := fresh "Ki" in
     let Ki' := fresh "Ki'" in
-    intros P_s σ_s ϕ e_s' σ_s' Hhead%prim_head_step;
+    intros ϕ e_s' σ_s' Hhead%prim_head_step;
     [inversion Hhead; subst; try by (apply ϕ; eauto)
     | intros K e' Heq Hv; clear ϕ;
       destruct K as [ | Ki K]; first (done);
@@ -43,8 +43,8 @@ Section irreducible.
         by rewrite -language_to_val_eq]
     ].
 
-  Global Instance irreducible_match v x1 e1 x2 e2 :
-    PureIrreducible (¬ ∃ v', v = InjLV v' ∨ v = InjRV v') (Match (Val v) x1 e1 x2 e2).
+  Global Instance irreducible_match v x1 e1 x2 e2 P σ :
+    SIrreducible (¬ ∃ v', v = InjLV v' ∨ v = InjRV v') P (Match (Val v) x1 e1 x2 e2) σ.
   Proof. prove_irred. Qed.
 
   (** for binary operators, we provide specialized instances for each operator.
@@ -61,58 +61,61 @@ Section irreducible.
         | H : _ ∧ _ |- _ => destruct H
         end; eauto 8.
 
-  Global Instance irreducible_plus v1 v2 :
-    PureIrreducible (¬ (∃ n, v1 = LitV $ LitInt n) ∨ ¬ (∃ n, v2 = LitV $ LitInt n))%V (BinOp PlusOp (Val v1) (Val v2)).
+  Global Instance irreducible_plus v1 v2 P σ :
+    SIrreducible (¬ (∃ n, v1 = LitV $ LitInt n) ∨ ¬ (∃ n, v2 = LitV $ LitInt n))%V P (BinOp PlusOp (Val v1) (Val v2)) σ.
   Proof. prove_irred. solve_binop v1 v2. Qed.
-  Global Instance irreducible_minus v1 v2 :
-    PureIrreducible (¬ (∃ n, v1 = LitV $ LitInt n) ∨ ¬ (∃ n, v2 = LitV $ LitInt n))%V (BinOp MinusOp (Val v1) (Val v2)).
+  Global Instance irreducible_minus v1 v2 P σ :
+    SIrreducible (¬ (∃ n, v1 = LitV $ LitInt n) ∨ ¬ (∃ n, v2 = LitV $ LitInt n))%V P (BinOp MinusOp (Val v1) (Val v2)) σ.
   Proof. prove_irred. solve_binop v1 v2. Qed.
-  Global Instance irreducible_rem v1 v2 :
-    PureIrreducible (¬ (∃ n, v1 = LitV $ LitInt n) ∨ ¬ (∃ n, v2 = LitV $ LitInt n))%V (BinOp RemOp (Val v1) (Val v2)).
+  Global Instance irreducible_rem v1 v2 P σ :
+    SIrreducible (¬ (∃ n, v1 = LitV $ LitInt n) ∨ ¬ (∃ n, v2 = LitV $ LitInt n))%V P (BinOp RemOp (Val v1) (Val v2)) σ.
   Proof. prove_irred. solve_binop v1 v2. Qed.
-  Global Instance irreducible_mult v1 v2 :
-    PureIrreducible (¬ (∃ n, v1 = LitV $ LitInt n) ∨ ¬ (∃ n, v2 = LitV $ LitInt n))%V (BinOp MultOp (Val v1) (Val v2)).
+  Global Instance irreducible_mult v1 v2 P σ :
+    SIrreducible (¬ (∃ n, v1 = LitV $ LitInt n) ∨ ¬ (∃ n, v2 = LitV $ LitInt n))%V P (BinOp MultOp (Val v1) (Val v2)) σ.
   Proof. prove_irred. solve_binop v1 v2. Qed.
-  Global Instance irreducible_quot v1 v2 :
-    PureIrreducible (¬ (∃ n, v1 = LitV $ LitInt n) ∨ ¬ (∃ n, v2 = LitV $ LitInt n))%V (BinOp QuotOp (Val v1) (Val v2)).
-  Proof. prove_irred. solve_binop v1 v2. Qed.
-
-  Global Instance irreducible_and v1 v2 :
-    PureIrreducible (¬ (((∃ n, v1 = LitV $ LitInt n) ∧ (∃ n, v2 = LitV $ LitInt n)) ∨ ((∃ b, v1 = LitV $ LitBool b) ∧ ∃ b, v2 = LitV $ LitBool b)))%V
-      (BinOp AndOp (Val v1) (Val v2)).
-  Proof. prove_irred. solve_binop v1 v2. Qed.
-  Global Instance irreducible_or v1 v2 :
-    PureIrreducible (¬ (((∃ n, v1 = LitV $ LitInt n) ∧ (∃ n, v2 = LitV $ LitInt n)) ∨ ((∃ b, v1 = LitV $ LitBool b) ∧ ∃ b, v2 = LitV $ LitBool b)))%V
-      (BinOp OrOp (Val v1) (Val v2)).
-  Proof. prove_irred. solve_binop v1 v2. Qed.
-  Global Instance irreducible_xor v1 v2 :
-    PureIrreducible (¬ (((∃ n, v1 = LitV $ LitInt n) ∧ (∃ n, v2 = LitV $ LitInt n)) ∨ ((∃ b, v1 = LitV $ LitBool b) ∧ ∃ b, v2 = LitV $ LitBool b)))%V
-      (BinOp XorOp (Val v1) (Val v2)).
+  Global Instance irreducible_quot v1 v2 P σ :
+    SIrreducible (¬ (∃ n, v1 = LitV $ LitInt n) ∨ ¬ (∃ n, v2 = LitV $ LitInt n))%V P (BinOp QuotOp (Val v1) (Val v2)) σ.
   Proof. prove_irred. solve_binop v1 v2. Qed.
 
-  Global Instance irreducible_shiftl v1 v2 :
-    PureIrreducible ((¬ (∃ n, v1 = LitV $ LitInt n)) ∨ (¬ (∃ n, v2 = LitV $ LitInt n)))%V
-      (BinOp ShiftLOp (Val v1) (Val v2)).
+  Global Instance irreducible_and v1 v2 P σ :
+    SIrreducible (¬ (((∃ n, v1 = LitV $ LitInt n) ∧ (∃ n, v2 = LitV $ LitInt n)) ∨ ((∃ b, v1 = LitV $ LitBool b) ∧ ∃ b, v2 = LitV $ LitBool b)))%V
+      P (BinOp AndOp (Val v1) (Val v2)) σ.
   Proof. prove_irred. solve_binop v1 v2. Qed.
-  Global Instance irreducible_shiftr v1 v2 :
-    PureIrreducible ((¬ (∃ n, v1 = LitV $ LitInt n)) ∨ (¬ (∃ n, v2 = LitV $ LitInt n)))%V
-      (BinOp ShiftROp (Val v1) (Val v2)).
+  Global Instance irreducible_or v1 v2 P σ :
+    SIrreducible (¬ (((∃ n, v1 = LitV $ LitInt n) ∧ (∃ n, v2 = LitV $ LitInt n)) ∨ ((∃ b, v1 = LitV $ LitBool b) ∧ ∃ b, v2 = LitV $ LitBool b)))%V
+      P (BinOp OrOp (Val v1) (Val v2)) σ.
   Proof. prove_irred. solve_binop v1 v2. Qed.
-
-  Global Instance irreducible_le v1 v2 :
-    PureIrreducible (¬ (∃ n, v1 = LitV $ LitInt n) ∨ ¬ (∃ n, v2 = LitV $ LitInt n))%V (BinOp LeOp (Val v1) (Val v2)).
-  Proof. prove_irred. solve_binop v1 v2. Qed.
-  Global Instance irreducible_ge v1 v2 :
-    PureIrreducible (¬ (∃ n, v1 = LitV $ LitInt n) ∨ ¬ (∃ n, v2 = LitV $ LitInt n))%V (BinOp LtOp (Val v1) (Val v2)).
+  Global Instance irreducible_xor v1 v2 P σ :
+    SIrreducible (¬ (((∃ n, v1 = LitV $ LitInt n) ∧ (∃ n, v2 = LitV $ LitInt n)) ∨ ((∃ b, v1 = LitV $ LitBool b) ∧ ∃ b, v2 = LitV $ LitBool b)))%V
+      P (BinOp XorOp (Val v1) (Val v2)) σ.
   Proof. prove_irred. solve_binop v1 v2. Qed.
 
-  Global Instance irreducible_offset v1 v2 :
-    PureIrreducible (¬ (∃ l, v1 = LitV $ LitLoc l) ∨ ¬ (∃ n, v2 = LitV $ LitInt n))%V (BinOp OffsetOp  (Val v1) (Val v2)).
+  Global Instance irreducible_shiftl v1 v2 P σ :
+    SIrreducible ((¬ (∃ n, v1 = LitV $ LitInt n)) ∨ (¬ (∃ n, v2 = LitV $ LitInt n)))%V
+      P (BinOp ShiftLOp (Val v1) (Val v2)) σ.
+  Proof. prove_irred. solve_binop v1 v2. Qed.
+  Global Instance irreducible_shiftr v1 v2 P σ :
+    SIrreducible ((¬ (∃ n, v1 = LitV $ LitInt n)) ∨ (¬ (∃ n, v2 = LitV $ LitInt n)))%V
+      P (BinOp ShiftROp (Val v1) (Val v2)) σ.
   Proof. prove_irred. solve_binop v1 v2. Qed.
 
-  Global Instance irreducible_eq v1 v2 :
-    PureIrreducible (¬ vals_compare_safe v1 v2)%V
-      (BinOp EqOp (Val v1) (Val v2)).
+  Global Instance irreducible_le v1 v2 P σ :
+    SIrreducible (¬ (∃ n, v1 = LitV $ LitInt n) ∨ ¬ (∃ n, v2 = LitV $ LitInt n))%V
+      P (BinOp LeOp (Val v1) (Val v2)) σ.
+  Proof. prove_irred. solve_binop v1 v2. Qed.
+  Global Instance irreducible_ge v1 v2 P σ :
+    SIrreducible (¬ (∃ n, v1 = LitV $ LitInt n) ∨ ¬ (∃ n, v2 = LitV $ LitInt n))%V
+      P (BinOp LtOp (Val v1) (Val v2)) σ.
+  Proof. prove_irred. solve_binop v1 v2. Qed.
+
+  Global Instance irreducible_offset v1 v2 P σ :
+    SIrreducible (¬ (∃ l, v1 = LitV $ LitLoc l) ∨ ¬ (∃ n, v2 = LitV $ LitInt n))%V
+      P (BinOp OffsetOp  (Val v1) (Val v2)) σ.
+  Proof. prove_irred. solve_binop v1 v2. Qed.
+
+  Global Instance irreducible_eq v1 v2 P σ :
+    SIrreducible (¬ vals_compare_safe v1 v2)%V
+      P (BinOp EqOp (Val v1) (Val v2)) σ.
   Proof.
     prove_irred.
     unfold bin_op_eval in *;
@@ -120,29 +123,38 @@ Section irreducible.
     case_decide; congruence.
   Qed.
 
-  Global Instance irreducible_unop v o :
-    PureIrreducible (¬ (is_Some $ un_op_eval o v)) (UnOp o (Val v)).
+  Global Instance irreducible_unop v o P σ :
+    SIrreducible (¬ (is_Some $ un_op_eval o v)) P (UnOp o (Val v)) σ.
   Proof. prove_irred. Qed.
 
-  Global Instance irreducible_var (x : string) :
-    PureIrreducible (True) (Var x).
+  Global Instance irreducible_var (x : string) P σ :
+    SIrreducible (True) P (Var x) σ.
   Proof. prove_irred. Qed.
 
-  Global Instance irreducible_call v v2 :
-    PureIrreducible (¬ ∃ fn, v = LitV $ LitFn fn) (Call (Val v) (Val v2)).
+  Global Instance irreducible_call v v2 P σ :
+    SIrreducible (¬ ∃ fn, v = LitV $ LitFn fn) P (Call (Val v) (Val v2)) σ.
   Proof. prove_irred. Qed.
 
-  Global Instance irreducible_if v e1 e2 :
-    PureIrreducible (¬ ∃ b, v = LitV $ LitBool b) (If (Val v) e1 e2).
+  Global Instance irreducible_if v e1 e2 P σ :
+    SIrreducible (¬ ∃ b, v = LitV $ LitBool b) P (If (Val v) e1 e2) σ.
   Proof. prove_irred. Qed.
 
-  Global Instance irreducible_fst v :
-    PureIrreducible (¬ ∃ v1 v2, v = PairV v1 v2) (Fst (Val v)).
+  Global Instance irreducible_fst v P σ :
+    SIrreducible (¬ ∃ v1 v2, v = PairV v1 v2) P (Fst (Val v)) σ.
   Proof. prove_irred. Qed.
-  Global Instance irreducible_snd v :
-    PureIrreducible (¬ ∃ v1 v2, v = PairV v1 v2) (Snd (Val v)).
+  Global Instance irreducible_snd v P σ :
+    SIrreducible (¬ ∃ v1 v2, v = PairV v1 v2) P (Snd (Val v)) σ.
   Proof. prove_irred. Qed.
 
+  Global Instance irreducible_load σ l P :
+    SIrreducible (¬ ∃ v, heap σ !! l = Some (Some v)) P (Load $ Val $ LitV $ LitLoc l) σ.
+  Proof. prove_irred. Qed.
+  Global Instance irreducible_store σ l P (v : val) :
+    SIrreducible (¬ ∃ v, heap σ !! l = Some (Some v)) P (Store (Val $ LitV $ LitLoc l) (Val v)) σ.
+  Proof. prove_irred. Qed.
+  Global Instance irreducible_free σ l P :
+    SIrreducible (¬ ∃ v, heap σ !! l = Some (Some v)) P (Free $ Val $ LitV $ LitLoc l) σ.
+  Proof. prove_irred. Qed.
 End irreducible.
 
 Section pure_exec.
